PREFIX cs: <https://linked.data.gov.au/def/tk-labels>
PREFIX dcterms: <http://purl.org/dc/terms/>
PREFIX lc: <https://linked.data.gov.au/def/lc/>
PREFIX owl: <http://www.w3.org/2002/07/owl#>
PREFIX rdfs: <http://www.w3.org/2000/01/rdf-schema#>
PREFIX sdo: <https://schema.org/>
PREFIX skos: <http://www.w3.org/2004/02/skos/core#>
PREFIX tk: <https://linked.data.gov.au/def/tk-labels/>
PREFIX xsd: <http://www.w3.org/2001/XMLSchema#>

cs:
    a skos:ConceptScheme ;
    dcterms:created "2022-06-22"^^xsd:date ;
    dcterms:creator <https://linked.data.gov.au/org/idn> ;
    dcterms:identifier "tk"^^xsd:token ;
    dcterms:modified "2022-06-22"^^xsd:date ;
    dcterms:provenance "This vocabulary was generated from the https://localcontexts.org website's content: https://localcontexts.org/labels/traditional-knowledge-labels/" ;
    dcterms:publisher <https://linked.data.gov.au/org/idn> ;
    dcterms:source "https://localcontexts.org/labels/traditional-knowledge-labels/"^^xsd:anyURI ;
    owl:versionInfo "1.0"^^xsd:string ;
    skos:definition "Traditional Knowledge (TK) labels \"support the inclusion of local protocols for access and use to cultural heritage that is digitally circulating outside community contexts\". This vocabulary is a SKOS-based listing of those labels so they can be accessed in RDF graph-based systems."@en ;
    skos:hasTopConcept
        tk:attribution ,
        tk:clan ,
        tk:commercial ,
        tk:community-use-only ,
        tk:community-voice ,
        tk:creative ,
        tk:culturally-sensitive ,
        tk:family ,
        tk:men-general ,
        tk:men-restricted ,
        tk:multiple-communities ,
        tk:non-commercial ,
        tk:non-verified ,
        tk:open-to-collaboration ,
        tk:outreach ,
        tk:seasonal ,
        tk:secret-sacred ,
        tk:verified ,
        tk:women-general ,
        tk:women-restricted ;
    skos:prefLabel "Traditional Knowledge Labels"@en ;
.

<https://linked.data.gov.au/org/idn>
    a sdo:Organization ;
    sdo:name "Indigenous Data Network" ;
    sdo:url "https://mspgh.unimelb.edu.au/centres-institutes/centre-for-health-equity/research-group/indigenous-data-network"^^xsd:anyURI ;
.

tk:attribution
    a
        skos:Concept ,
        lc:TKLabel ;
    dcterms:identifier "attribution"^^xsd:token ;
    dcterms:source "https://localcontexts.org/label/tk-attribution/"^^xsd:anyURI ;
    rdfs:isDefinedBy cs: ;
    skos:definition "This Label should be used when you would like anyone who uses this material to know who the correct sources, custodians, or owners are. This is especially useful if this material has been wrongly attributed or important names of the people involved in making this material or safeguarding this material, are missing. This Label allows you to correct historical mistakes in terms of naming and acknowledging the legitimate authorities for this material. This Label asks for future users to also apply the correct names and attribution."@en ;
    skos:inScheme cs: ;
    skos:notation "TK A" ;
    skos:prefLabel "Attribution"@en ;
.

tk:clan
    a
        skos:Concept ,
        lc:TKLabel ;
    dcterms:identifier "clan"^^xsd:token ;
    dcterms:source "https://localcontexts.org/label/tk-clan/"^^xsd:anyURI ;
    rdfs:isDefinedBy cs: ;
    skos:definition "This Label should be used when you would like external users to know that this material is subject to conditions for circulation relating to clan membership and/or is according to protocols for clan relationships. Because these conditions have not historically been recognized, this Label helps make these conditions for use and circulation clearer. Specifically, the Label asks future users to respect culturally specific rules of use and to make informed decisions about using this type of material."@en ;
    skos:inScheme cs: ;
    skos:notation "TK CL" ;
    skos:prefLabel "Clan"@en ;
.

tk:commercial
    a
        skos:Concept ,
        lc:TKLabel ;
    dcterms:identifier "commercial"^^xsd:token ;
    dcterms:source "https://localcontexts.org/label/tk-commercial/"^^xsd:anyURI ;
    rdfs:isDefinedBy cs: ;
    skos:definition "Communities have the right to benefit commercially from the information that is derived from their traditional knowledge. This Label is being used to indicate an expressed interest in being a primary party to any future negotiations if commercialization opportunities arise."@en ;
    skos:inScheme cs: ;
    skos:notation "TK OC" ;
    skos:prefLabel "Commercial"@en ;
.

tk:community-use-only
    a
        skos:Concept ,
        lc:TKLabel ;
    dcterms:identifier "community-use-only"^^xsd:token ;
    dcterms:source "https://localcontexts.org/label/tk-community-use-only/"^^xsd:anyURI ;
    rdfs:isDefinedBy cs: ;
    skos:definition "This Label should be used when you would like external users to know that this material is subject to certain conditions of circulation namely that this material is usually not circulated beyond the family, clan or community. Because these conditions have not historically been recognized, this Label helps make these conditions clearer for future users. Specifically it asks them to respect culturally specific rules of use and to make different and fair decisions about using this type of material."@en ;
    skos:inScheme cs: ;
    skos:notation "TK CO" ;
    skos:prefLabel "Community Use Only"@en ;
.

tk:community-voice
    a
        skos:Concept ,
        lc:TKLabel ;
    dcterms:identifier "community-voice"^^xsd:token ;
    dcterms:source "https://localcontexts.org/label/tk-community-voice/"^^xsd:anyURI ;
    rdfs:isDefinedBy cs: ;
    skos:definition "This Label should be used when you would like to encourage community members to share their knowledge, stories and experiences. This Label would usually be used within a community-based archive to encourage the sharing of stories. This Label indicates that the current narrative or explanation that accompanies this material is incomplete or partial and that many community voices are needed to help make sense of and understand the event, photograph, recording or heritage item. The Community Voice Label encourages multiplicity in the telling, listening and sharing of community histories and cultural knowledge."@en ;
    skos:inScheme cs: ;
    skos:notation "TK CV" ;
    skos:prefLabel "Community Voice"@en ;
.

tk:creative
    a
        skos:Concept ,
        lc:TKLabel ;
    dcterms:identifier "creative"^^xsd:token ;
    dcterms:source "https://localcontexts.org/label/tk-creative/"^^xsd:anyURI ;
    rdfs:isDefinedBy cs: ;
    skos:definition "This Label should be used when an individual artist or author would like to clearly connect creative practices with traditional knowledge deriving from their own community. While an individual artist or author has standard copyright and creative commons licenses available to use, this Label helps make clear that a creative practice is also deeply connected to a collective responsibility around the use and sharing of traditional knowledge."@en ;
    skos:inScheme cs: ;
    skos:notation "TK CR" ;
    skos:prefLabel "Creative"@en ;
.

tk:culturally-sensitive
    a
        skos:Concept ,
        lc:TKLabel ;
    dcterms:identifier "culturally-sensitive"^^xsd:token ;
    dcterms:source "https://localcontexts.org/label/tk-culturally-sensitive/"^^xsd:anyURI ;
    rdfs:isDefinedBy cs: ;
    skos:definition "This Label should be used when you would like external users to know that this material has special sensitivities around it and should be treated with great care. These sensitivities could include: that it has only recently been reconnected with the community from which it originates, that the community is currently vetting and spending time with the material, and/or that the material is culturally valued and needs to be kept safe. This Label could also be used to indicate that there are cultural sensitivities around this material arising from legacies of colonialism, for instance, the use of derogatory language or descriptive errors within the content and/or content descriptions."@en ;
    skos:inScheme cs: ;
    skos:notation "TK CS" ;
    skos:prefLabel "Culturally Sensitive"@en ;
.

tk:family
    a
        skos:Concept ,
        lc:TKLabel ;
    dcterms:identifier "family"^^xsd:token ;
    dcterms:source "https://localcontexts.org/label/tk-family/"^^xsd:anyURI ;
    rdfs:isDefinedBy cs: ;
    skos:definition "This Label should be used when you would like external users to know that this material is subject to certain conditions for circulation. This material is usually only shared between family members. Because these conditions have not historically been recognized, this Label helps make these conditions clearer for future users. Specifically it asks them to respect culturally specific rules of use and to make different and fair decisions about using this type of material."@en ;
    skos:inScheme cs: ;
    skos:notation "TK F" ;
    skos:prefLabel "Family"@en ;
.

tk:men-general
    a
        skos:Concept ,
        lc:TKLabel ;
    dcterms:identifier "men-general"^^xsd:token ;
    dcterms:source "https://localcontexts.org/label/tk-men-general/"^^xsd:anyURI ;
    rdfs:isDefinedBy cs: ;
    skos:definition "This Label should be used when you want to let external users know that the material circulating should only be shared between men in the community. This is a Men’s General Label and indicates that there are restrictions of access and use to men based on customary law. This Label can be used to help external users recognize that with this material there are specific protocols and conditions of use. This Label is designed to recognize that some knowledge is gendered, and that certain knowledge can only be shared among specific members of the community. It should be used to complement already existing customs and protocols of access and use."@en ;
    skos:inScheme cs: ;
    skos:notation "TK MG" ;
    skos:prefLabel "Men General"@en ;
.

tk:men-restricted
    a
        skos:Concept ,
        lc:TKLabel ;
    dcterms:identifier "men-restricted"^^xsd:token ;
    dcterms:source "https://localcontexts.org/label/tk-men-restricted/"^^xsd:anyURI ;
    rdfs:isDefinedBy cs: ;
    skos:definition "This Label should be used when you want to let external users know that the material circulating freely is actually of a highly restricted nature. This is a Men’s Highly Restricted Label and indicates that there are restrictions of access and use based on customary law. This Label can be used to help external users recognize that with this material there are very specific protocols and conditions of use. This Label is designed to recognize that some knowledge is gendered, and that certain knowledge expressions can only be shared among specific members of the community. Only authorized [and/or initiated] men within the community should be using this material."@en ;
    skos:inScheme cs: ;
    skos:notation "TK MR" ;
    skos:prefLabel "Men Restricted"@en ;
.

tk:multiple-communities
    a
        skos:Concept ,
        lc:TKLabel ;
    dcterms:identifier "multiple-communities"^^xsd:token ;
    dcterms:source "https://localcontexts.org/label/tk-multiple-communities/"^^xsd:anyURI ;
    rdfs:isDefinedBy cs: ;
    skos:definition "This Label should be used to indicate that multiple communities have responsibilities of custodianship and/or ownership over specific material. This Label recognizes that no singular community has explicit control. Rather, rights and responsibilities for use are spread across communities through already existing community protocols and ongoing cultural relationships."@en ;
    skos:inScheme cs: ;
    skos:notation "TK MC" ;
    skos:prefLabel "Multiple Communities"@en ;
.

tk:non-commercial
    a
        skos:Concept ,
        lc:TKLabel ;
    dcterms:identifier "non-commercial"^^xsd:token ;
    dcterms:source "https://localcontexts.org/label/tk-non-commercial/"^^xsd:anyURI ;
    rdfs:isDefinedBy cs: ;
    skos:definition "This Label should be used when you would like to let external users who have access to your material know that it should only be used in non-commercial ways. You are asking users to be respectful and fair with your cultural materials and ask that it not be used to derive economic benefits or used in any way that makes it into a commodity for sale or purchase."@en ;
    skos:inScheme cs: ;
    skos:notation "TK NC" ;
    skos:prefLabel "Non-Commercial"@en ;
.

tk:non-verified
    a
        skos:Concept ,
        lc:TKLabel ;
    dcterms:identifier "non-verified"^^xsd:token ;
    dcterms:source "https://localcontexts.org/label/tk-non-verified/"^^xsd:anyURI ;
    rdfs:isDefinedBy cs: ;
    skos:definition "This material has not been verified by the community. Reasons for this could include that it has not been appropriately vetted, has mistakes, omissions, derogatory language, lack of informed consent, or its process of creation was through dishonest research which did not follow proper community protocols."@en ;
    skos:inScheme cs: ;
    skos:notation "TK NV" ;
    skos:prefLabel "Non-Verified"@en ;
.

tk:open-to-collaboration
    a
        skos:Concept ,
        lc:TKLabel ;
    dcterms:identifier "open-to-collaboration"^^xsd:token ;
    dcterms:source "https://localcontexts.org/label/tk-open-to-collaboration/"^^xsd:anyURI ;
    rdfs:isDefinedBy cs: ;
    skos:definition "This Label is being used to indicate that the community is open to research collaborations. With this Label, future opportunities for collaboration and engagement are supported."@en ;
    skos:inScheme cs: ;
    skos:notation "TK CB" ;
    skos:prefLabel "Open To Collaboration"@en ;
.

tk:outreach
    a
        skos:Concept ,
        lc:TKLabel ;
    dcterms:identifier "outreach"^^xsd:token ;
    dcterms:source "https://localcontexts.org/label/tk-outreach/"^^xsd:anyURI ;
    rdfs:isDefinedBy cs: ;
    skos:definition "This Label should be used when you would only like your cultural materials used for educational outreach activities. Outreach activities means to share works outside the community in order to increase and raise awareness and education about your family, clan and/or community. Sites for outreach activities can include schools, universities, libraries, archives, museums, online forums, and small learning groups. Depending on what kind of context and the possibilities for increased circulation of this material, this Label helps TK holders and users to develop new possibilities in the fair and equitable reciprocal exchange for use of this material in outreach activities. This exchange might include access to educational or other resources that your community has difficulty accessing under other circumstances."@en ;
    skos:inScheme cs: ;
    skos:notation "TK O" ;
    skos:prefLabel "Outreach"@en ;
.

tk:seasonal
    a
        skos:Concept ,
        lc:TKLabel ;
    dcterms:identifier "seasonal"^^xsd:token ;
    dcterms:source "https://localcontexts.org/label/tk-seasonal/"^^xsd:anyURI ;
    rdfs:isDefinedBy cs: ;
    skos:definition "This Label should be used when you want to let external users know that the material that is openly circulating has seasonal conditions of access and use. This could mean that some material should only be used and heard at particular times of the year. It could also mean that the environment and land where this material derives also influences and impacts its meaning and significance. This Label can be used to help external users know that there are land-based teachings in this material which affect proper use and respectful understanding."@en ;
    skos:inScheme cs: ;
    skos:notation "TK S" ;
    skos:prefLabel "Seasonal"@en ;
.

tk:secret-sacred
    a
        skos:Concept ,
        lc:TKLabel ;
    dcterms:identifier "secret-sacred"^^xsd:token ;
    dcterms:source "https://localcontexts.org/label/tk-secret-sacred/"^^xsd:anyURI ;
    rdfs:isDefinedBy cs: ;
    skos:definition "This Label should be used when you want to let external users know that the material that is openly circulating contains secret/sacred information and that it has specific conditions of access and use. These conditions potentially include restrictions upon access. Using this Label helps to alert external users that this material is special and requires respectful and careful treatment. It asks users to make different decisions about using it and, importantly, to discuss any potential use with you."@en ;
    skos:inScheme cs: ;
    skos:notation "TK SS" ;
    skos:prefLabel "Secret Sacred"@en ;
.

tk:verified
    a
        skos:Concept ,
        lc:TKLabel ;
    dcterms:identifier "verified"^^xsd:token ;
    dcterms:source "https://localcontexts.org/label/tk-verified/"^^xsd:anyURI ;
    rdfs:isDefinedBy cs: ;
    skos:definition "This Label should be used when you and your community are satisfied with the way in which your traditional knowledge materials are being represented online or offline. This Label affirms that appropriate conditions for access and use are in place and that whoever has made this material accessible has made accommodations for cultural protocols associated with the knowledge. It lets users know that the right thing is being done by your community protocols and standards."@en ;
    skos:inScheme cs: ;
    skos:notation "TK V" ;
    skos:prefLabel "Verified"@en ;
.

tk:women-general
    a
        skos:Concept ,
        lc:TKLabel ;
    dcterms:identifier "women-general"^^xsd:token ;
    dcterms:source "https://localcontexts.org/label/tk-women-general/"^^xsd:anyURI ;
    rdfs:isDefinedBy cs: ;
    skos:definition "This Label should be used when you want to let external users know that the material circulating should only be shared between women in the community. This is a Women’s General Label and indicates that there are restrictions of access and use to women within the community based on customary law. This Label can be used to help external users recognize that with this material there are specific protocols and conditions of use. This Label is designed to recognize that some knowledge is gendered, and that certain knowledge can only be shared among specific members of the community. It should be used to complement already existing customs and protocols of access and use."@en ;
    skos:inScheme cs: ;
    skos:notation "TK WG" ;
    skos:prefLabel "Women General"@en ;
.

tk:women-restricted
    a
        skos:Concept ,
        lc:TKLabel ;
    dcterms:identifier "women-restricted"^^xsd:token ;
    dcterms:source "https://localcontexts.org/label/tk-women-restricted/"^^xsd:anyURI ;
    rdfs:isDefinedBy cs: ;
    skos:definition "This Label should be used when you want to let external users know that the material circulating freely is actually of a highly restricted nature. This is a Women’s Highly Restricted Label and indicates that there are restrictions of access and use based on customary law. This Label can be used to help external users recognize that with this material there are very specific protocols and conditions of use. This Label is designed to recognize that some knowledge is gendered, and that certain knowledge expressions can only be shared among specific members of the community. Only authorized [and/or initiated] women within the community should be using this material."@en ;
    skos:inScheme cs: ;
    skos:notation "TK WR" ;
    skos:prefLabel "Women Restricted"@en ;
.

<https://linked.data.gov.au/org/idn>
    a sdo:Organization ;
    sdo:name "Indigenous Data Network" ;
    sdo:url "https://www.idnau.org"^^xsd:anyURI ;
.
